open import Data.Nat using (â„•; zero; suc; _+_)
open import Relation.Binary.PropositionalEquality using (_â‰¡_; refl; cong)
open import Relation.Nullary using (Â¬_)
open import Data.Empty using (âŠ¥; âŠ¥-elim)
open import Data.Product using (Î£; _,_; âˆƒ; Î£-syntax; âˆƒ-syntax)

-- Inductive term definition from the book
data ğ•‹ : Set where
  true   : ğ•‹
  false  : ğ•‹
  zero   : ğ•‹
  suc    : ğ•‹ â†’ ğ•‹
  pred   : ğ•‹ â†’ ğ•‹
  iszero : ğ•‹ â†’ ğ•‹
  if_then_else_ : ğ•‹ â†’ ğ•‹ â†’ ğ•‹ â†’ ğ•‹

-- Inductive functions can be defined easily on an inductive definition of our terms

-- A rather weird and inefficient way
-- to define max but doesn't require any comparison
-- and suffices for the following depth function
max : â„• â†’ â„• â†’ â„•
max zero n = n
max (suc m) zero = suc m
max (suc m) (suc n) = suc (max m n)

-- Corresponds to the amount of nodes of the abstract syntax tree
size : ğ•‹ â†’ â„•
size true = 1
size false = 1
size zero = 1
size (suc t) = (size t) + 1
size (pred t) = (size t) + 1
size (iszero t) = (size t) + 1
size (if t then tâ‚ else tâ‚‚) = (size t) + (size tâ‚) + (size tâ‚‚) + 1

-- Corresponds to the first index of the set that the term appears in
-- within the constructive definition of our terms (see notes)
depth : ğ•‹ â†’ â„•
depth true = 1
depth false = 1
depth zero = 1
depth (suc t) = depth t + 1
depth (pred t) = depth t + 1
depth (iszero t) = depth t + 1
depth (if t then tâ‚ else tâ‚‚) = max (max (depth t) (depth tâ‚)) (depth tâ‚‚) + 1

-- Small step semantics of the toy language
data NValue : ğ•‹ â†’ Set where
  V-zero : NValue zero
  V-suc  : âˆ€ {t} â†’ NValue t â†’ NValue (suc t)

data Value : ğ•‹ â†’ Set where
  V-true  : Value true
  V-false : Value false
  V-num   : âˆ€ {t} â†’ NValue t â†’ Value t

infix 4 _â€”â†’_
data _â€”â†’_ : ğ•‹ â†’ ğ•‹ â†’ Set where
  Î¾-if     : âˆ€ {t t' tâ‚ tâ‚‚} â†’ t â€”â†’ t' â†’ if t then tâ‚ else tâ‚‚ â€”â†’ if t' then tâ‚ else tâ‚‚
  Î²-true   : âˆ€ {tâ‚ tâ‚‚} â†’ if true then tâ‚ else tâ‚‚ â€”â†’ tâ‚
  Î²-false  : âˆ€ {tâ‚ tâ‚‚} â†’ if false then tâ‚ else tâ‚‚ â€”â†’ tâ‚‚
  Î¾-suc    : âˆ€ {t t'} â†’ t â€”â†’ t' â†’ suc t â€”â†’ suc t'
  Î¾-pred   : âˆ€ {t t'} â†’ t â€”â†’ t' â†’ pred t â€”â†’ pred t'
  Î²-pred   : âˆ€ {t} â†’ NValue t â†’ pred (suc t) â€”â†’ t
  Î²-predz  : pred zero â€”â†’ zero
  Î¾-iszero : âˆ€ {t t'} â†’ t â€”â†’ t' â†’ iszero t â€”â†’ iszero t'
  Î²-zero   : iszero zero â€”â†’ true
  Î²-nv     : âˆ€ {t} â†’ NValue t â†’ iszero (suc t) â€”â†’ false

-- We can now do proofs about our semantics

-- Evaluation is deterministic

-- Lemma: Values do not step
Â¬valâ€”â†’t : âˆ€ {t t'} â†’ Value t â†’ Â¬ (t â€”â†’ t')
Â¬valâ€”â†’t V-true = Î»{ ()}
Â¬valâ€”â†’t V-false = Î»{ ()}
Â¬valâ€”â†’t (V-num V-zero) = Î»{ ()}
Â¬valâ€”â†’t (V-num (V-suc x)) = Î»{ (Î¾-suc xâ‚) â†’ Â¬valâ€”â†’t (V-num x) xâ‚}

determinacy : âˆ€ {t t' t''} â†’ t â€”â†’ t' â†’ t â€”â†’ t'' â†’ t' â‰¡ t'' 
determinacy (Î¾-if {tâ‚ = tâ‚} {tâ‚‚} tâ€”â†’t') (Î¾-if tâ€”â†’t'') = cong (Î» x â†’ if x then tâ‚ else tâ‚‚) (determinacy tâ€”â†’t' tâ€”â†’t'')
determinacy Î²-true Î²-true = refl
determinacy Î²-false Î²-false = refl
determinacy (Î¾-suc tâ€”â†’t') (Î¾-suc tâ€”â†’t'') = cong suc (determinacy tâ€”â†’t' tâ€”â†’t'')
determinacy (Î¾-pred tâ€”â†’t') (Î¾-pred tâ€”â†’t'') = cong pred (determinacy tâ€”â†’t' tâ€”â†’t'')
determinacy (Î¾-pred tâ€”â†’t') (Î²-pred x) = âŠ¥-elim (Â¬valâ€”â†’t (V-num (V-suc x)) tâ€”â†’t')
determinacy (Î²-pred x) (Î¾-pred tâ€”â†’t'') = âŠ¥-elim (Â¬valâ€”â†’t (V-num (V-suc x)) tâ€”â†’t'')
determinacy (Î²-pred x) (Î²-pred xâ‚) = refl
determinacy Î²-predz Î²-predz = refl
determinacy (Î¾-iszero tâ€”â†’t') (Î¾-iszero tâ€”â†’t'') = cong iszero (determinacy tâ€”â†’t' tâ€”â†’t'')
determinacy (Î¾-iszero tâ€”â†’t') (Î²-nv x) = âŠ¥-elim (Â¬valâ€”â†’t (V-num (V-suc x)) tâ€”â†’t')
determinacy Î²-zero Î²-zero = refl
determinacy (Î²-nv x) (Î¾-iszero tâ€”â†’t'') = âŠ¥-elim (Â¬valâ€”â†’t (V-num (V-suc x)) tâ€”â†’t'')
determinacy (Î²-nv x) (Î²-nv xâ‚) = refl

-------------------------------------------------------------------------------------------------------------------------------------------------

-- We can also define the transitive and reflexive closure
-- of our small step relation

infix 4 _â€”â†’*_
data _â€”â†’*_ : ğ•‹ â†’ ğ•‹ â†’ Set where
  â€”â†’*-refl : âˆ€ {t} â†’ t â€”â†’* t
  â€”â†’*-step : âˆ€ {t tâ‚ tâ‚‚} â†’ t â€”â†’ tâ‚ â†’ tâ‚ â€”â†’* tâ‚‚ â†’ t â€”â†’* tâ‚‚

-- The closure is transitive

â€”â†’*-trans : âˆ€ {t tâ‚ tâ‚‚} â†’ t â€”â†’* tâ‚ â†’ tâ‚ â€”â†’* tâ‚‚ â†’ t â€”â†’* tâ‚‚
â€”â†’*-trans â€”â†’*-refl tâ‚â€”â†’*tâ‚‚ = tâ‚â€”â†’*tâ‚‚
â€”â†’*-trans (â€”â†’*-step x tâ€”â†’*tâ‚) tâ‚â€”â†’*tâ‚‚ = â€”â†’*-step x (â€”â†’*-trans tâ€”â†’*tâ‚ tâ‚â€”â†’*tâ‚‚)

-------------------------------------------------------------------------------------------------------------------------------------------------

-- Big-step semantics
data NValue' : Set where
  zero : NValue'
  suc  : NValue' â†’ NValue'

data Value' : Set where
  num   : NValue' â†’ Value'
  true  : Value'
  false : Value'

âŒœ_âŒ : NValue' â†’ Value'
âŒœ zero âŒ = num zero
âŒœ suc nv âŒ = num (suc nv)

âŒ_âŒŸâ‚™ : NValue' â†’ ğ•‹
âŒ zero âŒŸâ‚™ = zero
âŒ suc nv âŒŸâ‚™ = suc âŒ nv âŒŸâ‚™

âŒ_âŒŸ : Value' â†’ ğ•‹
âŒ num x âŒŸ = âŒ x âŒŸâ‚™
âŒ true âŒŸ = true
âŒ false âŒŸ = false

NV'â†’NV : âˆ€ (nv : NValue') â†’ NValue âŒ nv âŒŸâ‚™
NV'â†’NV zero = V-zero
NV'â†’NV (suc nv) = V-suc (NV'â†’NV nv)

infix 4 _â‡“_
data _â‡“_ : ğ•‹ â†’ Value' â†’ Set where
  â‡“-zero       : zero â‡“ num zero
  â‡“-true       : true â‡“ true
  â‡“-false      : false â‡“ false
  â‡“-ifTrue     : âˆ€ {tâ‚ tâ‚‚ tâ‚ƒ vâ‚‚} â†’ tâ‚ â‡“ true â†’ tâ‚‚ â‡“ vâ‚‚ â†’ if tâ‚ then tâ‚‚ else tâ‚ƒ â‡“ vâ‚‚
  â‡“-ifFalse    : âˆ€ {tâ‚ tâ‚‚ tâ‚ƒ vâ‚ƒ} â†’ tâ‚ â‡“ false â†’ tâ‚ƒ â‡“ vâ‚ƒ â†’ if tâ‚ then tâ‚‚ else tâ‚ƒ â‡“ vâ‚ƒ
  â‡“-suc        : âˆ€ {t nv} â†’ t â‡“ num nv â†’  suc t â‡“ (num (suc nv))
  â‡“-predZero   : âˆ€ {t} â†’ t â‡“ num zero â†’ pred t â‡“ num zero
  â‡“-predSuc    : âˆ€ {t nv} â†’ t â‡“ num (suc nv) â†’ pred t â‡“ num nv
  â‡“-isZeroZero : âˆ€ {t} â†’ t â‡“ num zero â†’ iszero t â‡“ true
  â‡“-isZeroSuc  : âˆ€ {t nv} â†’ t â‡“ num (suc nv) â†’ iszero t â‡“ false

-- Semantic equivalence can be shown

-- â‡“ to â€”â†’*
Î¾-ifâ‚* : âˆ€ {tâ‚ tâ‚' tâ‚‚ tâ‚ƒ} â†’ tâ‚ â€”â†’* tâ‚' â†’ if tâ‚ then tâ‚‚ else tâ‚ƒ â€”â†’* if tâ‚' then tâ‚‚ else tâ‚ƒ
Î¾-ifâ‚* â€”â†’*-refl = â€”â†’*-refl
Î¾-ifâ‚* (â€”â†’*-step x tâ‚â€”â†’*tâ‚') = â€”â†’*-trans (â€”â†’*-step (Î¾-if x) â€”â†’*-refl) (Î¾-ifâ‚* tâ‚â€”â†’*tâ‚')

Î¾-suc* : âˆ€ {t t'} â†’ t â€”â†’* t' â†’ suc t â€”â†’* suc t'
Î¾-suc* â€”â†’*-refl = â€”â†’*-refl
Î¾-suc* (â€”â†’*-step x tâ€”â†’*t') = â€”â†’*-trans (â€”â†’*-step (Î¾-suc x) â€”â†’*-refl) (Î¾-suc* tâ€”â†’*t')

Î¾-pred* : âˆ€ {t t'} â†’ t â€”â†’* t' â†’ pred t â€”â†’* pred t'
Î¾-pred* â€”â†’*-refl = â€”â†’*-refl
Î¾-pred* (â€”â†’*-step x tâ€”â†’*t') = â€”â†’*-trans (â€”â†’*-step (Î¾-pred x) â€”â†’*-refl) (Î¾-pred* tâ€”â†’*t')

Î²-pred* : âˆ€ {t} â†’ t â€”â†’* zero â†’ pred t â€”â†’* zero
Î²-pred* â€”â†’*-refl = â€”â†’*-step Î²-predz â€”â†’*-refl
Î²-pred* (â€”â†’*-step x tâ€”â†’*z) = â€”â†’*-trans (â€”â†’*-step (Î¾-pred x) â€”â†’*-refl) (Î²-pred* tâ€”â†’*z)

Î¾-iszero* : âˆ€ {t t'} â†’ t â€”â†’* t' â†’ iszero t â€”â†’* iszero t'
Î¾-iszero* â€”â†’*-refl = â€”â†’*-refl
Î¾-iszero* (â€”â†’*-step x tâ€”â†’*t') = â€”â†’*-trans (â€”â†’*-step (Î¾-iszero x) â€”â†’*-refl) (Î¾-iszero* tâ€”â†’*t')

Î²-true* : âˆ€ {t} â†’ t â€”â†’* zero â†’ iszero t â€”â†’* true
Î²-true* â€”â†’*-refl = â€”â†’*-step Î²-zero â€”â†’*-refl
Î²-true* (â€”â†’*-step x tâ€”â†’*z) = â€”â†’*-trans (â€”â†’*-step (Î¾-iszero x) â€”â†’*-refl) (Î²-true* tâ€”â†’*z)

â‡“-â€”â†’* : âˆ€ {t v} â†’ t â‡“ v â†’ t â€”â†’* âŒ v âŒŸ
â‡“-â€”â†’* â‡“-zero = â€”â†’*-refl
â‡“-â€”â†’* â‡“-true = â€”â†’*-refl
â‡“-â€”â†’* â‡“-false = â€”â†’*-refl
â‡“-â€”â†’* (â‡“-ifTrue tâ‡“v tâ‡“vâ‚) = â€”â†’*-trans (Î¾-ifâ‚* (â‡“-â€”â†’* tâ‡“v)) (â€”â†’*-trans (â€”â†’*-step Î²-true â€”â†’*-refl) (â‡“-â€”â†’* tâ‡“vâ‚))
â‡“-â€”â†’* (â‡“-ifFalse tâ‡“v tâ‡“vâ‚) = â€”â†’*-trans (Î¾-ifâ‚* (â‡“-â€”â†’* tâ‡“v)) (â€”â†’*-trans (â€”â†’*-step Î²-false â€”â†’*-refl) (â‡“-â€”â†’* tâ‡“vâ‚))
â‡“-â€”â†’* (â‡“-suc tâ‡“v) = â€”â†’*-trans (Î¾-suc* (â‡“-â€”â†’* tâ‡“v)) â€”â†’*-refl
â‡“-â€”â†’* (â‡“-predZero tâ‡“v) = Î²-pred* (â‡“-â€”â†’* tâ‡“v) 
â‡“-â€”â†’* (â‡“-predSuc {nv = nv} tâ‡“v) = â€”â†’*-trans (Î¾-pred* (â‡“-â€”â†’* tâ‡“v)) (â€”â†’*-step (Î²-pred (NV'â†’NV nv)) â€”â†’*-refl)
â‡“-â€”â†’* (â‡“-isZeroZero tâ‡“v) = Î²-true* (â‡“-â€”â†’* tâ‡“v)
â‡“-â€”â†’* (â‡“-isZeroSuc {nv = nv} tâ‡“v) = â€”â†’*-trans (Î¾-iszero* (â‡“-â€”â†’* tâ‡“v)) (â€”â†’*-step (Î²-nv (NV'â†’NV nv)) â€”â†’*-refl)

-- â€”â†’* to â‡“
â‡“-refl-helper : âˆ€ {nv} â†’ âŒ nv âŒŸâ‚™ â‡“ num nv
â‡“-refl-helper {zero} = â‡“-zero
â‡“-refl-helper {suc nv} = â‡“-suc â‡“-refl-helper

â‡“-refl : âˆ€ {v} â†’ âŒ v âŒŸ â‡“ v
â‡“-refl {num x} = â‡“-refl-helper
â‡“-refl {true} = â‡“-true
â‡“-refl {false} = â‡“-false

val-lemma : âˆ€ {t} (nv : NValue t) â†’ âˆƒ[ V ] ( t â‰¡ âŒ V âŒŸâ‚™)
val-lemma V-zero = zero , refl
val-lemma (V-suc nv) with val-lemma nv
... | fst , refl = (suc fst) , refl

â€”â†’-â‡“-ext : âˆ€ {t t' v} â†’ t â€”â†’ t' â†’ t' â‡“ v â†’ t â‡“ v
â€”â†’-â‡“-ext Î²-true â‡“-zero = â‡“-ifTrue â‡“-true â‡“-zero
â€”â†’-â‡“-ext Î²-false â‡“-zero = â‡“-ifFalse â‡“-false â‡“-zero
â€”â†’-â‡“-ext (Î²-pred x) â‡“-zero = â‡“-predSuc (â‡“-suc â‡“-zero)
â€”â†’-â‡“-ext Î²-predz â‡“-zero = â‡“-predZero â‡“-zero
â€”â†’-â‡“-ext Î²-true â‡“-true = â‡“-ifTrue â‡“-true â‡“-true
â€”â†’-â‡“-ext Î²-false â‡“-true = â‡“-ifFalse â‡“-false â‡“-true
â€”â†’-â‡“-ext Î²-zero â‡“-true = â‡“-isZeroZero â‡“-zero
â€”â†’-â‡“-ext Î²-true â‡“-false = â‡“-ifTrue â‡“-true â‡“-false
â€”â†’-â‡“-ext Î²-false â‡“-false = â‡“-ifFalse â‡“-false â‡“-false
â€”â†’-â‡“-ext (Î²-nv x) â‡“-false with val-lemma x
... | fst , refl = â‡“-isZeroSuc (â‡“-suc â‡“-refl)
â€”â†’-â‡“-ext (Î¾-if tâ€”â†’t') (â‡“-ifTrue t'â‡“v t'â‡“vâ‚) = â‡“-ifTrue (â€”â†’-â‡“-ext tâ€”â†’t' t'â‡“v) t'â‡“vâ‚
â€”â†’-â‡“-ext Î²-true (â‡“-ifTrue t'â‡“v t'â‡“vâ‚) = â‡“-ifTrue â‡“-true (â‡“-ifTrue t'â‡“v t'â‡“vâ‚)
â€”â†’-â‡“-ext Î²-false (â‡“-ifTrue t'â‡“v t'â‡“vâ‚) = â‡“-ifFalse â‡“-false (â‡“-ifTrue t'â‡“v t'â‡“vâ‚)
â€”â†’-â‡“-ext (Î¾-if tâ€”â†’t') (â‡“-ifFalse t'â‡“v t'â‡“vâ‚) = â‡“-ifFalse (â€”â†’-â‡“-ext tâ€”â†’t' t'â‡“v) t'â‡“vâ‚
â€”â†’-â‡“-ext Î²-true (â‡“-ifFalse t'â‡“v t'â‡“vâ‚) = â‡“-ifTrue â‡“-true (â‡“-ifFalse t'â‡“v t'â‡“vâ‚)
â€”â†’-â‡“-ext Î²-false (â‡“-ifFalse t'â‡“v t'â‡“vâ‚) = â‡“-ifFalse â‡“-false (â‡“-ifFalse t'â‡“v t'â‡“vâ‚)
â€”â†’-â‡“-ext Î²-true (â‡“-suc t'â‡“v) = â‡“-ifTrue â‡“-true (â‡“-suc t'â‡“v)
â€”â†’-â‡“-ext Î²-false (â‡“-suc t'â‡“v) = â‡“-ifFalse â‡“-false (â‡“-suc t'â‡“v)
â€”â†’-â‡“-ext (Î¾-suc tâ€”â†’t') (â‡“-suc t'â‡“v) = â‡“-suc (â€”â†’-â‡“-ext tâ€”â†’t' t'â‡“v)
â€”â†’-â‡“-ext (Î²-pred x) (â‡“-suc t'â‡“v) = â‡“-predSuc (â‡“-suc (â‡“-suc t'â‡“v))
â€”â†’-â‡“-ext Î²-true (â‡“-predZero t'â‡“v) = â‡“-ifTrue â‡“-true (â‡“-predZero t'â‡“v)
â€”â†’-â‡“-ext Î²-false (â‡“-predZero t'â‡“v) = â‡“-ifFalse â‡“-false (â‡“-predZero t'â‡“v)
â€”â†’-â‡“-ext (Î¾-pred tâ€”â†’t') (â‡“-predZero t'â‡“v) = â‡“-predZero (â€”â†’-â‡“-ext tâ€”â†’t' t'â‡“v)
â€”â†’-â‡“-ext Î²-true (â‡“-predSuc t'â‡“v) = â‡“-ifTrue â‡“-true (â‡“-predSuc t'â‡“v)
â€”â†’-â‡“-ext Î²-false (â‡“-predSuc t'â‡“v) = â‡“-ifFalse â‡“-false (â‡“-predSuc t'â‡“v)
â€”â†’-â‡“-ext (Î¾-pred tâ€”â†’t') (â‡“-predSuc t'â‡“v) = â‡“-predSuc (â€”â†’-â‡“-ext tâ€”â†’t' t'â‡“v)
â€”â†’-â‡“-ext Î²-true (â‡“-isZeroZero t'â‡“v) = â‡“-ifTrue â‡“-true (â‡“-isZeroZero t'â‡“v)
â€”â†’-â‡“-ext Î²-false (â‡“-isZeroZero t'â‡“v) = â‡“-ifFalse â‡“-false (â‡“-isZeroZero t'â‡“v)
â€”â†’-â‡“-ext (Î¾-iszero tâ€”â†’t') (â‡“-isZeroZero t'â‡“v) = â‡“-isZeroZero (â€”â†’-â‡“-ext tâ€”â†’t' t'â‡“v)
â€”â†’-â‡“-ext Î²-true (â‡“-isZeroSuc t'â‡“v) = â‡“-ifTrue â‡“-true (â‡“-isZeroSuc t'â‡“v)
â€”â†’-â‡“-ext Î²-false (â‡“-isZeroSuc t'â‡“v) = â‡“-ifFalse â‡“-false (â‡“-isZeroSuc t'â‡“v)
â€”â†’-â‡“-ext (Î¾-iszero tâ€”â†’t') (â‡“-isZeroSuc t'â‡“v) = â‡“-isZeroSuc (â€”â†’-â‡“-ext tâ€”â†’t' t'â‡“v)

â€”â†’*-â‡“ : âˆ€ {t v} â†’ t â€”â†’* âŒ v âŒŸ â†’ t â‡“ v
â€”â†’*-â‡“ â€”â†’*-refl = â‡“-refl
â€”â†’*-â‡“ (â€”â†’*-step x tâ€”â†’*v) = â€”â†’-â‡“-ext x (â€”â†’*-â‡“ tâ€”â†’*v)
